Seccompjit.v
@@ -1,61 +1,12 @@
-Require Import compcert.backend.RTL.
+Require Import compcert.backend.Cminor.
 Require Import compcert.common.AST.
 Require Import compcert.common.Errors.
 Require Import compcert.lib.Coqlib.
 Require Import compcert.lib.Integers.
 Require Import compcert.lib.Maps.
-Require Import Op.
 Require Import Seccomp.
 
 Parameter seccomp_memwords: Z.
-
-Record state: Type := mkstate {
-  st_code: RTL.code;
-  st_ep: node;
-  st_map: ZMap.t node
-}.
-
-Record fnmap: Type := mkfnmap {
-  fn: RTL.function;
-  map: ZMap.t node
-}.
-
-Inductive state_incr: state -> state -> Prop :=
-  state_incr_intro:
-    forall (s1 s2: state),
-    Ple s1.(st_ep) s2.(st_ep) ->
-    (forall pc,
-      s1.(st_code)!pc = None \/ s2.(st_code)!pc = s1.(st_code)!pc) ->
-    state_incr s1 s2.
-
-Lemma state_incr_refl:
-  forall s, state_incr s s.
-Proof.
-  intros.
-  apply state_incr_intro.
-  apply Ple_refl.
-  intros; auto.
-Qed.
-
-Lemma state_incr_trans:
-  forall s1 s2 s3, state_incr s1 s2 -> state_incr s2 s3 -> state_incr s1 s3.
-Proof.
-  intros.
-  inv H; inv H0.
-  apply state_incr_intro.
-  apply Ple_trans with s2.(st_ep); assumption.
-
-  intros.
-  generalize (H2 pc) (H3 pc).
-  intuition congruence.
-Qed.
-
-Definition add_instr (instr: RTL.instruction) (st: state) : state :=
-  let n := Psucc st.(st_ep) in
-  mkstate (PTree.set n instr st.(st_code)) n st.(st_map).
-
-Definition add_map (pc: Z) (st: state) : state :=
-  mkstate st.(st_code) st.(st_ep) (ZMap.set pc st.(st_ep) st.(st_map)).
 
 Definition reg_a:   ident := 1%positive.
 Definition reg_x:   ident := 2%positive.
@@ -63,42 +14,46 @@ Definition reg_mem: ident := 3%positive.
 
 Open Local Scope error_monad_scope.
 
-Definition transl_instr (instr: Seccomp.instruction) (pc: Z) (st: state) : res state :=
+Definition transl_instr (instr: Seccomp.instruction) : res Cminor.stmt :=
   match instr with
   | Salu_add_k k =>
-    OK (add_instr (Iop (Oaddimm k) (reg_a::nil) reg_a st.(st_ep)) st)
+    OK (Sassign reg_a (Ebinop Oadd (Evar reg_a) (Econst (Ointconst k))))
   | Sret_a =>
-    OK (add_instr (Ireturn (Some reg_a)) st)
+    OK (Sreturn (Some (Evar reg_a)))
   | _ => Error (msg "FIXME")
   end.
 
-Fixpoint transl_code (src: Seccomp.code) (pc: Z) (st: state) : res state :=
-  match src with
-  | nil => OK st
+Fixpoint transl_code (c: Seccomp.code) : res Cminor.stmt :=
+  match c with
+  | nil => OK Sskip
   | hd::tl =>
-    do st <- transl_code tl (Zsucc pc) st;
-    do st <- transl_instr hd pc st;
-    OK (add_map pc st)
+    do t <- transl_code tl;
+    do h <- transl_instr hd;
+    OK (Sseq h t)
   end.
 
-Definition transl_function (f: Seccomp.function) : res fnmap :=
-  let st := mkstate (PTree.empty RTL.instruction) 1%positive (ZMap.init 1%positive) in
-  do st <- transl_code f 0 st;
-  let sig := mksignature nil (Some Tint) in
-  let stacksize := (Zmult seccomp_memwords 4) in
+Definition transl_funbody (f: Seccomp.function) : res Cminor.stmt :=
+  do b <- transl_code f;
   (* FIXME: memset(mem, 0, sizeof(mem)) *)
-  let st := add_instr (Iop (Oaddrstack Int.zero) nil reg_mem st.(st_ep)) st in
-  let st := add_instr (Iop (Ointconst Int.zero) nil reg_x st.(st_ep)) st in
-  let st := add_instr (Iop (Ointconst Int.zero) nil reg_a st.(st_ep)) st in
-  OK (mkfnmap (RTL.mkfunction sig nil stacksize st.(st_code) st.(st_ep)) st.(st_map)).
+  let init_a := (Sassign reg_a (Econst (Ointconst Int.zero))) in
+  let init_x := (Sassign reg_x (Econst (Ointconst Int.zero))) in
+  let init_mem := (Sassign reg_mem (Econst (Oaddrstack Int.zero))) in
+  OK (Sseq init_a (Sseq init_x (Sseq init_mem b))).
+
+Definition transl_function (f: Seccomp.function) : res Cminor.function :=
+  do body <- transl_funbody f;
+  let sig := mksignature nil (Some Tint) in
+  let vars := reg_a::reg_x::reg_mem::nil in
+  let stackspace := (Zmult seccomp_memwords 4) in
+  OK (Cminor.mkfunction sig nil vars stackspace body).
 
 Local Open Scope string_scope.
 
 Definition transl_fundef (fd: fundef) :=
   match fd with
-  | Internal f => do f' <- transl_function f; OK (Internal f'.(fn))
+  | Internal f => do f' <- transl_function f; OK (Internal f')
   | External ef => Error (msg "no external function allowed")
   end.
 
-Definition transl_program (p: Seccomp.program) : res RTL.program :=
+Definition transl_program (p: Seccomp.program) : res Cminor.program :=
   transform_partial_program transl_fundef p.
