Makefile
@@ -26,4 +26,4 @@ codegen/extraction.vo: $(FILES:.v=.vo)
 
 clean:
 	rm -rf _build *.vo *.glob *.native
-	cd codegen && rm -f *.ml *.mlo *.glob
+	cd codegen && rm -f *.ml *.mli *.mlo *.glob *.vo
